Refactor message equality.  Sill have final no model step propagation lemma to prove

KeyManagement/Simulation.v
@@ -56,24 +56,52 @@ Inductive chan_key : Set :=
     -> chan_key
 .
 
-Inductive action_matches : forall {A B : type},
-                           RealWorld.action -> RealWorld.universe A B ->
-                           IdealWorld.action -> IdealWorld.universe A -> Prop :=
-| Inp : forall A B t (m__rw : RealWorld.crypto t) (m__iw m__expected : IdealWorld.message.message t)
-               ms (U__rw : RealWorld.universe A B) (U__iw : IdealWorld.universe A) rw iw ch_id cs ps p froms,
-      rw = (RealWorld.Input m__rw p froms)
-      -> iw = IdealWorld.Input m__iw ch_id cs ps
-      -> U__iw.(IdealWorld.channel_vector) #? ch_id = Some ((existT _ _ m__expected) :: ms)
-      -> MessageEq.message_eq m__rw U__rw m__iw U__iw ch_id
-      -> action_matches rw U__rw iw U__iw
-| Out : forall A B t (m__rw : RealWorld.crypto t) (m__iw : IdealWorld.message.message t)
-          (U__rw : RealWorld.universe A B) (U__iw : IdealWorld.universe A) rw iw ch_id cs ps suid_to suid_from sents,
-    rw = RealWorld.Output m__rw suid_to suid_from sents
-    -> iw = IdealWorld.Output m__iw ch_id cs ps
-    (* -> U__iw.(IdealWorld.channel_vector) $? ch_id = Some (ms ++ [existT _ _ m__expected]) *)
-    -> MessageEq.message_eq m__rw U__rw m__iw U__iw ch_id
-    -> action_matches rw U__rw iw U__iw
+Inductive action_matches (cs : RealWorld.ciphers) (gks : keys) :
+  RealWorld.action -> IdealWorld.action -> Prop :=
+
+| InpSig : forall t (m__rw : RealWorld.crypto t) (msg__rw : RealWorld.message.message t) (m__iw : IdealWorld.message.message t)
+          kid uid seq froms p cid ch_id chans ps,
+    m__rw = RealWorld.SignedCiphertext cid
+    -> cs $? cid = Some (RealWorld.SigCipher kid uid seq msg__rw)
+    -> content_eq msg__rw m__iw gks
+    -> action_matches cs gks (RealWorld.Input m__rw p froms) (IdealWorld.Input m__iw ch_id chans ps)
+| InpEnc : forall t (m__rw : RealWorld.crypto t) (msg__rw : RealWorld.message.message t) (m__iw : IdealWorld.message.message t)
+          kid1 kid2 uid seq froms p cid ch_id chans ps,
+    m__rw = RealWorld.SignedCiphertext cid
+    -> cs $? cid = Some (RealWorld.SigEncCipher kid1 kid2 uid seq msg__rw)
+    -> content_eq msg__rw m__iw gks
+    -> action_matches cs gks (RealWorld.Input m__rw p froms) (IdealWorld.Input m__iw ch_id chans ps)
+| OutSig : forall t (m__rw : RealWorld.crypto t) (msg__rw : RealWorld.message.message t) (m__iw : IdealWorld.message.message t)
+          kid uid seq to from sents cid ch_id chans ps,
+    m__rw = RealWorld.SignedCiphertext cid
+    -> cs $? cid = Some (RealWorld.SigCipher kid uid seq msg__rw)
+    -> content_eq msg__rw m__iw gks
+    -> action_matches cs gks (RealWorld.Output m__rw to from sents) (IdealWorld.Output m__iw ch_id chans ps)
+| OutEnc : forall t (m__rw : RealWorld.crypto t) (msg__rw : RealWorld.message.message t) (m__iw : IdealWorld.message.message t)
+          kid1 kid2 uid seq to from sents cid ch_id chans ps,
+    m__rw = RealWorld.SignedCiphertext cid
+    -> cs $? cid = Some (RealWorld.SigEncCipher kid1 kid2 uid seq msg__rw)
+    -> content_eq msg__rw m__iw gks
+    -> action_matches cs gks (RealWorld.Output m__rw to from sents) (IdealWorld.Output m__iw ch_id chans ps)
 .
+
+(* Inductive action_matches : forall {A B : type}, *)
+(*                            RealWorld.action -> RealWorld.universe A B -> *)
+(*                            IdealWorld.action -> IdealWorld.universe A -> Prop := *)
+(* | Inp : forall A B t (m__rw : RealWorld.crypto t) (m__iw m__expected : IdealWorld.message.message t) *)
+(*                ms (U__rw : RealWorld.universe A B) (U__iw : IdealWorld.universe A) rw iw ch_id cs ps p froms, *)
+(*       rw = (RealWorld.Input m__rw p froms) *)
+(*       -> iw = IdealWorld.Input m__iw ch_id cs ps *)
+(*       -> U__iw.(IdealWorld.channel_vector) #? ch_id = Some ((existT _ _ m__expected) :: ms) *)
+(*       -> MessageEq.message_eq m__rw U__rw m__iw U__iw ch_id *)
+(*       -> action_matches rw U__rw iw U__iw *)
+(* | Out : forall A B t (m__rw : RealWorld.crypto t) (m__iw : IdealWorld.message.message t) *)
+(*           (U__rw : RealWorld.universe A B) (U__iw : IdealWorld.universe A) rw iw ch_id cs ps suid_to suid_from sents, *)
+(*     rw = RealWorld.Output m__rw suid_to suid_from sents *)
+(*     -> iw = IdealWorld.Output m__iw ch_id cs ps *)
+(*     -> MessageEq.message_eq m__rw U__rw m__iw U__iw ch_id *)
+(*     -> action_matches rw U__rw iw U__iw *)
+(* . *)
 
 Section RealWorldUniverseProperties.
   Import RealWorld.
@@ -405,12 +433,12 @@ Section Simulation.
     -> universe_ok U__r
     -> adv_universe_ok U__r
     -> advP U__r.(RealWorld.adversary)
-    -> forall a1 U__r',
-        RealWorld.step_universe U__r (Messages.Action a1) U__r' (* excludes adversary steps *)
-        -> exists a2 U__i' U__i'',
+    -> forall ra U__r',
+        RealWorld.step_universe U__r (Messages.Action ra) U__r' (* excludes adversary steps *)
+        -> exists ia U__i' U__i'',
           istepSilent^* U__i U__i'
-        /\ IdealWorld.lstep_universe U__i' (Messages.Action a2) U__i''
-        /\ action_matches a1 U__r a2 U__i'
+        /\ IdealWorld.lstep_universe U__i' (Messages.Action ia) U__i''
+        /\ action_matches U__r.(RealWorld.all_ciphers) U__r.(RealWorld.all_keys) ra ia
         /\ R (RealWorld.peel_adv U__r') U__i''.
 
   Definition honest_actions_safe :=
