protocols/RealWorldStepLemmas.v
@@ -576,97 +576,97 @@ Section MessageEqLemmas.
       rewrite RW; eauto.
   Qed.
 
-  Lemma message_eq_user_add_nochange_cs_ks_msgs :
-    forall A B (usrs : honest_users A) (adv adv' : user_data B) cs gks
-      ks cmd qmsgs mycs froms sents cur_n cmd' sents' cur_n'
-      t (m__rw : crypto t) m__iw iu chid uid,
+  (* Lemma message_eq_user_add_nochange_cs_ks_msgs : *)
+  (*   forall A B (usrs : honest_users A) (adv adv' : user_data B) cs gks *)
+  (*     ks cmd qmsgs mycs froms sents cur_n cmd' sents' cur_n' *)
+  (*     t (m__rw : crypto t) m__iw iu chid uid, *)
 
-      usrs $? uid = Some (mkUserData ks cmd qmsgs mycs froms sents cur_n)
-      -> message_eq m__rw {| users := usrs; adversary := adv; all_ciphers := cs; all_keys := gks |} m__iw iu chid
-      -> message_eq
-          m__rw
-          {| users :=
-               usrs $+ (uid,
-                        {| key_heap := ks;
-                           protocol := cmd';
-                           msg_heap := qmsgs;
-                           c_heap := mycs;
-                           from_nons := froms;
-                           sent_nons := sents';
-                           cur_nonce := cur_n' |});
-             adversary := adv';
-             all_ciphers := cs;
-             all_keys := gks |} m__iw iu chid.
-  Proof using All.
-    intros.
+  (*     usrs $? uid = Some (mkUserData ks cmd qmsgs mycs froms sents cur_n) *)
+  (*     -> message_eq m__rw {| users := usrs; adversary := adv; all_ciphers := cs; all_keys := gks |} m__iw iu chid *)
+  (*     -> message_eq *)
+  (*         m__rw *)
+  (*         {| users := *)
+  (*              usrs $+ (uid, *)
+  (*                       {| key_heap := ks; *)
+  (*                          protocol := cmd'; *)
+  (*                          msg_heap := qmsgs; *)
+  (*                          c_heap := mycs; *)
+  (*                          from_nons := froms; *)
+  (*                          sent_nons := sents'; *)
+  (*                          cur_nonce := cur_n' |}); *)
+  (*            adversary := adv'; *)
+  (*            all_ciphers := cs; *)
+  (*            all_keys := gks |} m__iw iu chid. *)
+  (* Proof using All. *)
+  (*   intros. *)
 
-    invert H0; [ econstructor 1 | econstructor 2 ]; simpl in *; eauto;
-      intros;
-      autorewrite with find_user_keys in *; eauto;
-        destruct (u ==n uid); subst; clean_map_lookups; eauto; simpl; eauto;
-          match goal with
-          | [ ARG : ?usrs $? ?uid = Some _,
-                    IARG : IdealWorld.users _ $? ?uid = Some _,
-                           H : (forall _ _ _, ?usrs $? _ = Some _ -> _) |- _ ] =>
-            eapply H in ARG
-          end; eauto.
+  (*   invert H0; [ econstructor 1 | econstructor 2 ]; simpl in *; eauto; *)
+  (*     intros; *)
+  (*     autorewrite with find_user_keys in *; eauto; *)
+  (*       destruct (u ==n uid); subst; clean_map_lookups; eauto; simpl; eauto; *)
+  (*         match goal with *)
+  (*         | [ ARG : ?usrs $? ?uid = Some _, *)
+  (*                   IARG : IdealWorld.users _ $? ?uid = Some _, *)
+  (*                          H : (forall _ _ _, ?usrs $? _ = Some _ -> _) |- _ ] => *)
+  (*           eapply H in ARG *)
+  (*         end; eauto. *)
 
-    all: 
-      invert H; [ econstructor 1 | econstructor 2 ]; eauto.
-  Qed.
+  (*   all:  *)
+  (*     invert H; [ econstructor 1 | econstructor 2 ]; eauto. *)
+  (* Qed. *)
 
-  Lemma message_eq_user_add_nochange_drop_not_signed_addressed_msg :
-    forall A B (usrs : honest_users A) (adv adv' : user_data B) cs gks
-      ks cmd t (msg : crypto t) qmsgs mycs froms sents cur_n cmd' sents' cur_n'
-      t (m__rw : crypto t) m__iw iu chid uid,
+  (* Lemma message_eq_user_add_nochange_drop_not_signed_addressed_msg : *)
+  (*   forall A B (usrs : honest_users A) (adv adv' : user_data B) cs gks *)
+  (*     ks cmd t (msg : crypto t) qmsgs mycs froms sents cur_n cmd' sents' cur_n' *)
+  (*     t (m__rw : crypto t) m__iw iu chid uid, *)
 
-      usrs $? uid = Some (mkUserData ks cmd (existT _ _ msg :: qmsgs) mycs froms sents cur_n)
-      -> msg_signed_addressed (findUserKeys usrs) cs (Some uid) msg = false
-      -> message_eq m__rw {| users := usrs; adversary := adv; all_ciphers := cs; all_keys := gks |} m__iw iu chid
-      -> message_eq
-          m__rw
-          {| users :=
-               usrs $+ (uid,
-                        {| key_heap := ks;
-                           protocol := cmd';
-                           msg_heap := qmsgs;
-                           c_heap := mycs;
-                           from_nons := froms;
-                           sent_nons := sents';
-                           cur_nonce := cur_n' |});
-             adversary := adv';
-             all_ciphers := cs;
-             all_keys := gks |} m__iw iu chid.
-  Proof.
-    intros.
+  (*     usrs $? uid = Some (mkUserData ks cmd (existT _ _ msg :: qmsgs) mycs froms sents cur_n) *)
+  (*     -> msg_signed_addressed (findUserKeys usrs) cs (Some uid) msg = false *)
+  (*     -> message_eq m__rw {| users := usrs; adversary := adv; all_ciphers := cs; all_keys := gks |} m__iw iu chid *)
+  (*     -> message_eq *)
+  (*         m__rw *)
+  (*         {| users := *)
+  (*              usrs $+ (uid, *)
+  (*                       {| key_heap := ks; *)
+  (*                          protocol := cmd'; *)
+  (*                          msg_heap := qmsgs; *)
+  (*                          c_heap := mycs; *)
+  (*                          from_nons := froms; *)
+  (*                          sent_nons := sents'; *)
+  (*                          cur_nonce := cur_n' |}); *)
+  (*            adversary := adv'; *)
+  (*            all_ciphers := cs; *)
+  (*            all_keys := gks |} m__iw iu chid. *)
+  (* Proof. *)
+  (*   intros. *)
 
-    assert ( KPMQ : key_perms_from_message_queue cs (findUserKeys usrs) (existT _ _ msg :: qmsgs) uid froms $0
-                    = key_perms_from_message_queue cs (findUserKeys usrs) qmsgs uid froms $0).
-    unfold key_perms_from_message_queue.
-    pose proof (clean_messages_cons_split cs (findUserKeys usrs) uid froms qmsgs _ _ msg eq_refl); split_ors; subst.
-    rewrite H2; trivial.
+  (*   assert ( KPMQ : key_perms_from_message_queue cs (findUserKeys usrs) (existT _ _ msg :: qmsgs) uid froms $0 *)
+  (*                   = key_perms_from_message_queue cs (findUserKeys usrs) qmsgs uid froms $0). *)
+  (*   unfold key_perms_from_message_queue. *)
+  (*   pose proof (clean_messages_cons_split cs (findUserKeys usrs) uid froms qmsgs _ _ msg eq_refl); split_ors; subst. *)
+  (*   rewrite H2; trivial. *)
 
-    unfold not_replayed, msg_signed_addressed in * |- .
-    rewrite andb_false_iff in H0; rewrite !andb_true_iff in H3; split_ex; split_ors.
-    rewrite H0 in H3; discriminate.
-    unfold msg_to_this_user, msg_destination_user in *; context_map_rewrites;
-      destruct (cipher_to_user x1 ==n uid); subst; discriminate.
+  (*   unfold not_replayed, msg_signed_addressed in * |- . *)
+  (*   rewrite andb_false_iff in H0; rewrite !andb_true_iff in H3; split_ex; split_ors. *)
+  (*   rewrite H0 in H3; discriminate. *)
+  (*   unfold msg_to_this_user, msg_destination_user in *; context_map_rewrites; *)
+  (*     destruct (cipher_to_user x1 ==n uid); subst; discriminate. *)
 
-    invert H1; [ econstructor 1 | econstructor 2 ]; simpl in *; eauto;
-      intros;
-      autorewrite with find_user_keys in *; eauto;
-        destruct (u ==n uid); subst; clean_map_lookups; eauto; simpl; eauto;
-          match goal with
-          | [ ARG : ?usrs $? ?uid = Some _,
-                    IARG : IdealWorld.users _ $? ?uid = Some _,
-                           H : (forall _ _ _, ?usrs $? _ = Some _ -> _) |- _ ] =>
-            eapply H in ARG
-          end; eauto.
+  (*   invert H1; [ econstructor 1 | econstructor 2 ]; simpl in *; eauto; *)
+  (*     intros; *)
+  (*     autorewrite with find_user_keys in *; eauto; *)
+  (*       destruct (u ==n uid); subst; clean_map_lookups; eauto; simpl; eauto; *)
+  (*         match goal with *)
+  (*         | [ ARG : ?usrs $? ?uid = Some _, *)
+  (*                   IARG : IdealWorld.users _ $? ?uid = Some _, *)
+  (*                          H : (forall _ _ _, ?usrs $? _ = Some _ -> _) |- _ ] => *)
+  (*           eapply H in ARG *)
+  (*         end; eauto. *)
 
-    all: 
-      invert H; [ econstructor 1 | econstructor 2 ]; simpl in *; eauto;
-      rewrite <- KPMQ; eauto.
-  Qed.
+  (*   all:  *)
+  (*     invert H; [ econstructor 1 | econstructor 2 ]; simpl in *; eauto; *)
+  (*     rewrite <- KPMQ; eauto. *)
+  (* Qed. *)
 
   (* Lemma message_eq_user_add_nochange_drop_signed_addressed_msg : *)
   (*   forall A B (usrs : honest_users A) (adv adv' : user_data B) cs gks *)
@@ -914,415 +914,415 @@ Section MessageEqLemmas.
     clean_map_lookups; eauto.
   Qed.
 
-  Lemma message_eq_user_add_addnl_cipher_inv :
-    forall A B (usrs : honest_users A) (adv adv' : user_data B) cs cs' cid c gks
-      ks  qmsgs mycs froms sents cur_n cmd cmd' sents' cur_n'
-      t (m__rw : crypto t) m__iw iu chid uid,
+  (* Lemma message_eq_user_add_addnl_cipher_inv : *)
+  (*   forall A B (usrs : honest_users A) (adv adv' : user_data B) cs cs' cid c gks *)
+  (*     ks  qmsgs mycs froms sents cur_n cmd cmd' sents' cur_n' *)
+  (*     t (m__rw : crypto t) m__iw iu chid uid, *)
 
-      ~ In cid cs
-      -> cs' = cs $+ (cid,c)
-      -> usrs $? uid = Some (mkUserData ks cmd qmsgs mycs froms sents cur_n)
-      (* -> encrypted_ciphers_ok (findUserKeys usrs) cs gks *)
-      -> user_cipher_queues_ok cs (findUserKeys usrs) usrs
-      -> message_queues_ok cs usrs gks
-      -> match c with
-        | @SigCipher t _ _ _ m | @SigEncCipher t _ _ _ _ m => keys_mine ks (findKeysMessage m)
-        end
-      -> (forall cid, msg_cipher_id m__rw = Some cid -> cs $? cid <> None)
-      -> message_eq
-          m__rw
-          {| users :=
-               usrs $+ (uid,
-                        {| key_heap := ks;
-                           protocol := cmd';
-                           msg_heap := qmsgs;
-                           c_heap := cid :: mycs;
-                           from_nons := froms;
-                           sent_nons := sents';
-                           cur_nonce := cur_n' |});
-             adversary := adv';
-             all_ciphers := cs';
-             all_keys := gks |} m__iw iu chid
-      -> message_eq m__rw {| users := usrs; adversary := adv; all_ciphers := cs; all_keys := gks |} m__iw iu chid.
-  Proof.
-    intros; subst.
-    assert (msg_cipher_id m__rw <> Some cid).
-    unfold not; intros MCID; eapply H5 in MCID; clean_map_lookups; contradiction.
+  (*     ~ In cid cs *)
+  (*     -> cs' = cs $+ (cid,c) *)
+  (*     -> usrs $? uid = Some (mkUserData ks cmd qmsgs mycs froms sents cur_n) *)
+  (*     (* -> encrypted_ciphers_ok (findUserKeys usrs) cs gks *) *)
+  (*     -> user_cipher_queues_ok cs (findUserKeys usrs) usrs *)
+  (*     -> message_queues_ok cs usrs gks *)
+  (*     -> match c with *)
+  (*       | @SigCipher t _ _ _ m | @SigEncCipher t _ _ _ _ m => keys_mine ks (findKeysMessage m) *)
+  (*       end *)
+  (*     -> (forall cid, msg_cipher_id m__rw = Some cid -> cs $? cid <> None) *)
+  (*     -> message_eq *)
+  (*         m__rw *)
+  (*         {| users := *)
+  (*              usrs $+ (uid, *)
+  (*                       {| key_heap := ks; *)
+  (*                          protocol := cmd'; *)
+  (*                          msg_heap := qmsgs; *)
+  (*                          c_heap := cid :: mycs; *)
+  (*                          from_nons := froms; *)
+  (*                          sent_nons := sents'; *)
+  (*                          cur_nonce := cur_n' |}); *)
+  (*            adversary := adv'; *)
+  (*            all_ciphers := cs'; *)
+  (*            all_keys := gks |} m__iw iu chid *)
+  (*     -> message_eq m__rw {| users := usrs; adversary := adv; all_ciphers := cs; all_keys := gks |} m__iw iu chid. *)
+  (* Proof. *)
+  (*   intros; subst. *)
+  (*   assert (msg_cipher_id m__rw <> Some cid). *)
+  (*   unfold not; intros MCID; eapply H5 in MCID; clean_map_lookups; contradiction. *)
 
-    invert H6; [ econstructor 1 | econstructor 2 ];
-      simpl in *;
-      autorewrite with find_user_keys in *;
-      eauto.
+  (*   invert H6; [ econstructor 1 | econstructor 2 ]; *)
+  (*     simpl in *; *)
+  (*     autorewrite with find_user_keys in *; *)
+  (*     eauto. *)
 
-    - intros.
-      specialize (H17 u); destruct (u ==n uid); subst; clean_map_lookups; eauto.
-      eapply H17 in H7; eauto.
-      invert H7; simpl in *; [ econstructor 1 | econstructor 2 ]; eauto;
-        simpl; clean_map_lookups.
-      msg_queue_prop.
-      user_cipher_queues_prop.
-      erewrite (* <- key_perms_from_message_queue_idempotent_addnl_cipher, *)
-               <- key_perms_from_known_ciphers_idempotent_addnl_cipher in H16 by eauto.
-      destruct c;
-        rewrite key_perms_from_known_ciphers_pull_merge ,
-                merge_perms_sym with (ks1 := key_perms_from_known_ciphers cs mycs $0),
-                <- merge_perms_assoc,
-                merge_keys_mine with (ks1 := ks) in H16 by eauto; eauto; simpl.
+  (*   - intros. *)
+  (*     specialize (H17 u); destruct (u ==n uid); subst; clean_map_lookups; eauto. *)
+  (*     eapply H17 in H7; eauto. *)
+  (*     invert H7; simpl in *; [ econstructor 1 | econstructor 2 ]; eauto; *)
+  (*       simpl; clean_map_lookups. *)
+  (*     msg_queue_prop. *)
+  (*     user_cipher_queues_prop. *)
+  (*     erewrite (* <- key_perms_from_message_queue_idempotent_addnl_cipher, *) *)
+  (*              <- key_perms_from_known_ciphers_idempotent_addnl_cipher in H16 by eauto. *)
+  (*     destruct c; *)
+  (*       rewrite key_perms_from_known_ciphers_pull_merge , *)
+  (*               merge_perms_sym with (ks1 := key_perms_from_known_ciphers cs mycs $0), *)
+  (*               <- merge_perms_assoc, *)
+  (*               merge_keys_mine with (ks1 := ks) in H16 by eauto; eauto; simpl. *)
 
-      eapply H17 in H7; eauto.
-      invert H7; simpl in *; [ econstructor 1 | econstructor 2 ]; eauto;
-        simpl; clean_map_lookups.
-      msg_queue_prop.
-      user_cipher_queues_prop.
-      erewrite (* <- key_perms_from_message_queue_idempotent_addnl_cipher, *)
-               <- key_perms_from_known_ciphers_idempotent_addnl_cipher in H18 by eauto; eauto.
+  (*     eapply H17 in H7; eauto. *)
+  (*     invert H7; simpl in *; [ econstructor 1 | econstructor 2 ]; eauto; *)
+  (*       simpl; clean_map_lookups. *)
+  (*     msg_queue_prop. *)
+  (*     user_cipher_queues_prop. *)
+  (*     erewrite (* <- key_perms_from_message_queue_idempotent_addnl_cipher, *) *)
+  (*              <- key_perms_from_known_ciphers_idempotent_addnl_cipher in H18 by eauto; eauto. *)
 
-    - intros.
-      specialize (H17 u); destruct (u ==n uid); subst; clean_map_lookups; eauto.
-      eapply H17 in H7; eauto.
+  (*   - intros. *)
+  (*     specialize (H17 u); destruct (u ==n uid); subst; clean_map_lookups; eauto. *)
+  (*     eapply H17 in H7; eauto. *)
 
-      invert H7; simpl in *; [ econstructor 1 | econstructor 2 ]; eauto;
-        simpl; clean_map_lookups; eauto
-        ; msg_queue_prop
-        ; user_cipher_queues_prop.
-      erewrite (* <- key_perms_from_message_queue_idempotent_addnl_cipher, *)
-               <- key_perms_from_known_ciphers_idempotent_addnl_cipher in H18 by eauto.
-      destruct c;
-        rewrite key_perms_from_known_ciphers_pull_merge ,
-                merge_perms_sym with (ks1 := key_perms_from_known_ciphers cs mycs $0),
-                <- merge_perms_assoc,
-                merge_keys_mine with (ks1 := ks) in H18 by eauto; eauto.
+  (*     invert H7; simpl in *; [ econstructor 1 | econstructor 2 ]; eauto; *)
+  (*       simpl; clean_map_lookups; eauto *)
+  (*       ; msg_queue_prop *)
+  (*       ; user_cipher_queues_prop. *)
+  (*     erewrite (* <- key_perms_from_message_queue_idempotent_addnl_cipher, *) *)
+  (*              <- key_perms_from_known_ciphers_idempotent_addnl_cipher in H18 by eauto. *)
+  (*     destruct c; *)
+  (*       rewrite key_perms_from_known_ciphers_pull_merge , *)
+  (*               merge_perms_sym with (ks1 := key_perms_from_known_ciphers cs mycs $0), *)
+  (*               <- merge_perms_assoc, *)
+  (*               merge_keys_mine with (ks1 := ks) in H18 by eauto; eauto. *)
 
-      erewrite (* <- key_perms_from_message_queue_idempotent_addnl_cipher, *)
-               <- key_perms_from_known_ciphers_idempotent_addnl_cipher in H19 by eauto.
-      destruct c;
-        rewrite key_perms_from_known_ciphers_pull_merge ,
-        merge_perms_sym with (ks1 := key_perms_from_known_ciphers cs mycs $0),
-                             <- merge_perms_assoc,
-                merge_keys_mine with (ks1 := ks) in H19 by eauto; eauto.
+  (*     erewrite (* <- key_perms_from_message_queue_idempotent_addnl_cipher, *) *)
+  (*              <- key_perms_from_known_ciphers_idempotent_addnl_cipher in H19 by eauto. *)
+  (*     destruct c; *)
+  (*       rewrite key_perms_from_known_ciphers_pull_merge , *)
+  (*       merge_perms_sym with (ks1 := key_perms_from_known_ciphers cs mycs $0), *)
+  (*                            <- merge_perms_assoc, *)
+  (*               merge_keys_mine with (ks1 := ks) in H19 by eauto; eauto. *)
 
-      eapply H17 in H7; eauto.
-      invert H7; simpl in *; [ econstructor 1 | econstructor 2 ]; eauto;
-        simpl; clean_map_lookups;
-          msg_queue_prop;
-          user_cipher_queues_prop.
+  (*     eapply H17 in H7; eauto. *)
+  (*     invert H7; simpl in *; [ econstructor 1 | econstructor 2 ]; eauto; *)
+  (*       simpl; clean_map_lookups; *)
+  (*         msg_queue_prop; *)
+  (*         user_cipher_queues_prop. *)
 
-      erewrite (* <- key_perms_from_message_queue_idempotent_addnl_cipher, *)
-               <- key_perms_from_known_ciphers_idempotent_addnl_cipher in H19 by eauto; eauto.
+  (*     erewrite (* <- key_perms_from_message_queue_idempotent_addnl_cipher, *) *)
+  (*              <- key_perms_from_known_ciphers_idempotent_addnl_cipher in H19 by eauto; eauto. *)
 
-      erewrite (* <- key_perms_from_message_queue_idempotent_addnl_cipher, *)
-               <- key_perms_from_known_ciphers_idempotent_addnl_cipher in H20; eauto.
-  Qed.
+  (*     erewrite (* <- key_perms_from_message_queue_idempotent_addnl_cipher, *) *)
+  (*              <- key_perms_from_known_ciphers_idempotent_addnl_cipher in H20; eauto. *)
+  (* Qed. *)
 
-  Lemma message_eq_user_add_addnl_cipher :
-    forall A B (usrs : honest_users A) (adv adv' : user_data B) cs cs' cid c gks
-      ks cmd qmsgs mycs froms sents cur_n cmd' sents' cur_n'
-      t (m__rw : crypto t) m__iw iu chid uid,
+  (* Lemma message_eq_user_add_addnl_cipher : *)
+  (*   forall A B (usrs : honest_users A) (adv adv' : user_data B) cs cs' cid c gks *)
+  (*     ks cmd qmsgs mycs froms sents cur_n cmd' sents' cur_n' *)
+  (*     t (m__rw : crypto t) m__iw iu chid uid, *)
 
-      ~ In cid cs
-      -> cs' = cs $+ (cid,c)
-      -> usrs $? uid = Some (mkUserData ks cmd qmsgs mycs froms sents cur_n)
-      -> encrypted_ciphers_ok (findUserKeys usrs) cs gks
-      -> user_cipher_queues_ok cs (findUserKeys usrs) usrs
-      -> message_queues_ok cs usrs gks
-      -> match c with
-        | @SigCipher t _ _ _ m | @SigEncCipher t _ _ _ _ m => keys_mine ks (findKeysMessage m)
-        end
-      -> message_eq m__rw {| users := usrs; adversary := adv; all_ciphers := cs; all_keys := gks |} m__iw iu chid
-      -> message_eq
-          m__rw
-          {| users :=
-               usrs $+ (uid,
-                        {| key_heap := ks;
-                           protocol := cmd';
-                           msg_heap := qmsgs;
-                           c_heap := cid :: mycs;
-                           from_nons := froms;
-                           sent_nons := sents';
-                           cur_nonce := cur_n' |});
-             adversary := adv';
-             all_ciphers := cs';
-             all_keys := gks |} m__iw iu chid.
-  Proof.
-    intros; subst.
+  (*     ~ In cid cs *)
+  (*     -> cs' = cs $+ (cid,c) *)
+  (*     -> usrs $? uid = Some (mkUserData ks cmd qmsgs mycs froms sents cur_n) *)
+  (*     -> encrypted_ciphers_ok (findUserKeys usrs) cs gks *)
+  (*     -> user_cipher_queues_ok cs (findUserKeys usrs) usrs *)
+  (*     -> message_queues_ok cs usrs gks *)
+  (*     -> match c with *)
+  (*       | @SigCipher t _ _ _ m | @SigEncCipher t _ _ _ _ m => keys_mine ks (findKeysMessage m) *)
+  (*       end *)
+  (*     -> message_eq m__rw {| users := usrs; adversary := adv; all_ciphers := cs; all_keys := gks |} m__iw iu chid *)
+  (*     -> message_eq *)
+  (*         m__rw *)
+  (*         {| users := *)
+  (*              usrs $+ (uid, *)
+  (*                       {| key_heap := ks; *)
+  (*                          protocol := cmd'; *)
+  (*                          msg_heap := qmsgs; *)
+  (*                          c_heap := cid :: mycs; *)
+  (*                          from_nons := froms; *)
+  (*                          sent_nons := sents'; *)
+  (*                          cur_nonce := cur_n' |}); *)
+  (*            adversary := adv'; *)
+  (*            all_ciphers := cs'; *)
+  (*            all_keys := gks |} m__iw iu chid. *)
+  (* Proof. *)
+  (*   intros; subst. *)
 
-    invert H6; [ econstructor 1 | econstructor 2 ]; simpl in *; eauto;
-      intros;
-      autorewrite with find_user_keys in *; eauto;
-        destruct (u ==n uid); subst; clean_map_lookups; eauto; simpl; eauto;
-          match goal with
-          | [ ARG : ?usrs $? ?uid = Some _,
-                    IARG : IdealWorld.users _ $? ?uid = Some _,
-                           H : (forall _ _ _, ?usrs $? _ = Some _ -> _) |- _ ] =>
-            generalize ARG; intros; eapply H in ARG
-          end; eauto;
-            destruct (c_id ==n cid); subst; clean_map_lookups.
+  (*   invert H6; [ econstructor 1 | econstructor 2 ]; simpl in *; eauto; *)
+  (*     intros; *)
+  (*     autorewrite with find_user_keys in *; eauto; *)
+  (*       destruct (u ==n uid); subst; clean_map_lookups; eauto; simpl; eauto; *)
+  (*         match goal with *)
+  (*         | [ ARG : ?usrs $? ?uid = Some _, *)
+  (*                   IARG : IdealWorld.users _ $? ?uid = Some _, *)
+  (*                          H : (forall _ _ _, ?usrs $? _ = Some _ -> _) |- _ ] => *)
+  (*           generalize ARG; intros; eapply H in ARG *)
+  (*         end; eauto; *)
+  (*           destruct (c_id ==n cid); subst; clean_map_lookups. *)
 
-    - invert H1; [ econstructor 1 | econstructor 2 ]; eauto; simpl in *; clean_map_lookups.
-      msg_queue_prop.
-      user_cipher_queues_prop.
-      (* erewrite <- key_perms_from_message_queue_idempotent_addnl_cipher; eauto. *)
-      assert (RW : key_perms_from_known_ciphers (cs $+ (cid, c)) (cid :: mycs) $0
-                   = key_perms_from_known_ciphers (cs $+ (cid, c)) mycs
-                                                  match c with
-                                                  | @SigCipher t0 _ _ _ m | @SigEncCipher t0 _ _ _ _ m => $0 $k++ findKeysMessage m
-                                                  end) by (simpl; clean_map_lookups; trivial).
-      rewrite <- RW; clear RW.
-      erewrite key_perms_from_known_ciphers_user_new_cipher; eauto.
-      rewrite merge_perms_sym with (ks1 := key_perms_from_known_ciphers cs mycs $0), <- merge_perms_assoc.
+  (*   - invert H1; [ econstructor 1 | econstructor 2 ]; eauto; simpl in *; clean_map_lookups. *)
+  (*     msg_queue_prop. *)
+  (*     user_cipher_queues_prop. *)
+  (*     (* erewrite <- key_perms_from_message_queue_idempotent_addnl_cipher; eauto. *) *)
+  (*     assert (RW : key_perms_from_known_ciphers (cs $+ (cid, c)) (cid :: mycs) $0 *)
+  (*                  = key_perms_from_known_ciphers (cs $+ (cid, c)) mycs *)
+  (*                                                 match c with *)
+  (*                                                 | @SigCipher t0 _ _ _ m | @SigEncCipher t0 _ _ _ _ m => $0 $k++ findKeysMessage m *)
+  (*                                                 end) by (simpl; clean_map_lookups; trivial). *)
+  (*     rewrite <- RW; clear RW. *)
+  (*     erewrite key_perms_from_known_ciphers_user_new_cipher; eauto. *)
+  (*     rewrite merge_perms_sym with (ks1 := key_perms_from_known_ciphers cs mycs $0), <- merge_perms_assoc. *)
 
-      Ltac go :=
-        match goal with
-        | [ H : ?ks1 $? ?k = Some ?x , CP : compat_perm (Some ?x) ?b |- compat_perm (?ks2 $? ?k) ?b ] =>
-          assert (RW: ks2 $? k = Some x)
+  (*     Ltac go := *)
+  (*       match goal with *)
+  (*       | [ H : ?ks1 $? ?k = Some ?x , CP : compat_perm (Some ?x) ?b |- compat_perm (?ks2 $? ?k) ?b ] => *)
+  (*         assert (RW: ks2 $? k = Some x) *)
 
-        | [ H : ?ks1 $? ?k = None , CP : compat_perm None ?b |- compat_perm (?ks2 $? ?k) ?b ] =>
-          idtac H CP
-        | [ H : compat_perm (?ks1 $? ?k) ?b |- compat_perm (?ks2 $? ?k) ?b ] =>
-          cases (ks1 $? k)
-        end.
+  (*       | [ H : ?ks1 $? ?k = None , CP : compat_perm None ?b |- compat_perm (?ks2 $? ?k) ?b ] => *)
+  (*         idtac H CP *)
+  (*       | [ H : compat_perm (?ks1 $? ?k) ?b |- compat_perm (?ks2 $? ?k) ?b ] => *)
+  (*         cases (ks1 $? k) *)
+  (*       end. *)
 
-      go; go.
-      eapply perm_merge_same with (ks1' := ks $k++ match c with
-                                                   | @SigCipher t0 _ _ _ m | @SigEncCipher t0 _ _ _ _ m => findKeysMessage m
-                                                   end); try eassumption; trivial; destruct c; rewrite merge_keys_mine; trivial.
-      rewrite RW; assumption.
+  (*     go; go. *)
+  (*     eapply perm_merge_same with (ks1' := ks $k++ match c with *)
+  (*                                                  | @SigCipher t0 _ _ _ m | @SigEncCipher t0 _ _ _ _ m => findKeysMessage m *)
+  (*                                                  end); try eassumption; trivial; destruct c; rewrite merge_keys_mine; trivial. *)
+  (*     rewrite RW; assumption. *)
 
-      repeat
-        match goal with
-        | [ H : _ $k++ _ $? _ = None |- _ ] => 
-          apply merge_perms_no_disappear_perms in H; split_ex
-        end.
+  (*     repeat *)
+  (*       match goal with *)
+  (*       | [ H : _ $k++ _ $? _ = None |- _ ] =>  *)
+  (*         apply merge_perms_no_disappear_perms in H; split_ex *)
+  (*       end. *)
 
-      Ltac xx :=
-        match goal with
-        | [ H : ?m $? ?k = None |- compat_perm (?ks1 $k++ ?m $k++ ?ks2 $k++ ?ks3 $? ?k) _ ] =>
-          let RW := fresh "RW"
-          in assert (RW: ks1 $k++ m $k++ ks2 $k++ ks3 $? k = None) by (repeat eapply merge_perms_adds_no_new_perms; eauto); rewrite RW
-        | [ |- compat_perm (_ $k++ ?m $k++ _ $k++ _ $? ?k) _ ] =>
-          assert (m $? k = None) by (repeat xx)
-        | [ |- (match ?c with _ => _ end) $? _ = None ] => destruct c
-        | [ H : keys_mine _ (findKeysMessage ?m) |- _ ] => unfold keys_mine in H
-        | [ H : (forall _ _, findKeysMessage _ $? _ = Some _ -> _)
-                , FK : findKeysMessage ?msg $? ?k = Some _ |- _ ] =>
-          eapply H in FK; split_ors; clean_map_lookups
-        | [ |- findKeysMessage ?msg $? ?k = None ] =>
-          cases (findKeysMessage msg $? k); auto
-        end.
+  (*     Ltac xx := *)
+  (*       match goal with *)
+  (*       | [ H : ?m $? ?k = None |- compat_perm (?ks1 $k++ ?m $k++ ?ks2 $k++ ?ks3 $? ?k) _ ] => *)
+  (*         let RW := fresh "RW" *)
+  (*         in assert (RW: ks1 $k++ m $k++ ks2 $k++ ks3 $? k = None) by (repeat eapply merge_perms_adds_no_new_perms; eauto); rewrite RW *)
+  (*       | [ |- compat_perm (_ $k++ ?m $k++ _ $k++ _ $? ?k) _ ] => *)
+  (*         assert (m $? k = None) by (repeat xx) *)
+  (*       | [ |- (match ?c with _ => _ end) $? _ = None ] => destruct c *)
+  (*       | [ H : keys_mine _ (findKeysMessage ?m) |- _ ] => unfold keys_mine in H *)
+  (*       | [ H : (forall _ _, findKeysMessage _ $? _ = Some _ -> _) *)
+  (*               , FK : findKeysMessage ?msg $? ?k = Some _ |- _ ] => *)
+  (*         eapply H in FK; split_ors; clean_map_lookups *)
+  (*       | [ |- findKeysMessage ?msg $? ?k = None ] => *)
+  (*         cases (findKeysMessage msg $? k); auto *)
+  (*       end. *)
 
-      repeat xx; eauto.
+  (*     repeat xx; eauto. *)
 
       
-    - invert H0; [ econstructor 1 | econstructor 2 ]; eauto; simpl in *; clean_map_lookups.
-      msg_queue_prop.
-      (* erewrite <- key_perms_from_message_queue_idempotent_addnl_cipher; eauto. *)
-      user_cipher_queues_prop.
-      erewrite <- key_perms_from_known_ciphers_idempotent_addnl_cipher; eauto.
+  (*   - invert H0; [ econstructor 1 | econstructor 2 ]; eauto; simpl in *; clean_map_lookups. *)
+  (*     msg_queue_prop. *)
+  (*     (* erewrite <- key_perms_from_message_queue_idempotent_addnl_cipher; eauto. *) *)
+  (*     user_cipher_queues_prop. *)
+  (*     erewrite <- key_perms_from_known_ciphers_idempotent_addnl_cipher; eauto. *)
 
-    - invert H1; [ econstructor 1 | econstructor 2 ]; eauto; simpl in *; clean_map_lookups;
-        msg_queue_prop;
-        user_cipher_queues_prop;
-        (* erewrite <- key_perms_from_message_queue_idempotent_addnl_cipher; *)
-        eauto.
+  (*   - invert H1; [ econstructor 1 | econstructor 2 ]; eauto; simpl in *; clean_map_lookups; *)
+  (*       msg_queue_prop; *)
+  (*       user_cipher_queues_prop; *)
+  (*       (* erewrite <- key_perms_from_message_queue_idempotent_addnl_cipher; *) *)
+  (*       eauto. *)
 
-      + assert (RW : key_perms_from_known_ciphers (cs $+ (cid, c)) (cid :: mycs) $0
-                     = key_perms_from_known_ciphers (cs $+ (cid, c)) mycs
-                                                    match c with
-                                                    | @SigCipher t0 _ _ _ m | @SigEncCipher t0 _ _ _ _ m => $0 $k++ findKeysMessage m
-                                                    end) by (simpl; clean_map_lookups; trivial).
-        rewrite <- RW; clear RW.
-        erewrite key_perms_from_known_ciphers_user_new_cipher; eauto.
-        rewrite merge_perms_sym with (ks1 := key_perms_from_known_ciphers cs mycs $0), <- merge_perms_assoc.
+  (*     + assert (RW : key_perms_from_known_ciphers (cs $+ (cid, c)) (cid :: mycs) $0 *)
+  (*                    = key_perms_from_known_ciphers (cs $+ (cid, c)) mycs *)
+  (*                                                   match c with *)
+  (*                                                   | @SigCipher t0 _ _ _ m | @SigEncCipher t0 _ _ _ _ m => $0 $k++ findKeysMessage m *)
+  (*                                                   end) by (simpl; clean_map_lookups; trivial). *)
+  (*       rewrite <- RW; clear RW. *)
+  (*       erewrite key_perms_from_known_ciphers_user_new_cipher; eauto. *)
+  (*       rewrite merge_perms_sym with (ks1 := key_perms_from_known_ciphers cs mycs $0), <- merge_perms_assoc. *)
 
-        go; go.
-        eapply perm_merge_same with (ks1' := ks $k++ match c with
-                                                     | @SigCipher t0 _ _ _ m | @SigEncCipher t0 _ _ _ _ m => findKeysMessage m
-                                                     end); try eassumption; trivial; destruct c; rewrite merge_keys_mine; trivial.
-        rewrite RW; assumption.
+  (*       go; go. *)
+  (*       eapply perm_merge_same with (ks1' := ks $k++ match c with *)
+  (*                                                    | @SigCipher t0 _ _ _ m | @SigEncCipher t0 _ _ _ _ m => findKeysMessage m *)
+  (*                                                    end); try eassumption; trivial; destruct c; rewrite merge_keys_mine; trivial. *)
+  (*       rewrite RW; assumption. *)
 
-        repeat
-          match goal with
-          | [ H : _ $k++ _ $? _ = None |- _ ] => 
-            apply merge_perms_no_disappear_perms in H; split_ex
-          end.
-        repeat xx; eauto.
+  (*       repeat *)
+  (*         match goal with *)
+  (*         | [ H : _ $k++ _ $? _ = None |- _ ] =>  *)
+  (*           apply merge_perms_no_disappear_perms in H; split_ex *)
+  (*         end. *)
+  (*       repeat xx; eauto. *)
         
-      + assert (RW : key_perms_from_known_ciphers (cs $+ (cid, c)) (cid :: mycs) $0
-                     = key_perms_from_known_ciphers (cs $+ (cid, c)) mycs
-                                                    match c with
-                                                    | @SigCipher t0 _ _ _ m | @SigEncCipher t0 _ _ _ _ m => $0 $k++ findKeysMessage m
-                                                    end) by (simpl; clean_map_lookups; trivial).
-        rewrite <- RW; clear RW.
-        erewrite key_perms_from_known_ciphers_user_new_cipher; eauto.
-        rewrite merge_perms_sym with (ks1 := key_perms_from_known_ciphers cs mycs $0), <- merge_perms_assoc.
+  (*     + assert (RW : key_perms_from_known_ciphers (cs $+ (cid, c)) (cid :: mycs) $0 *)
+  (*                    = key_perms_from_known_ciphers (cs $+ (cid, c)) mycs *)
+  (*                                                   match c with *)
+  (*                                                   | @SigCipher t0 _ _ _ m | @SigEncCipher t0 _ _ _ _ m => $0 $k++ findKeysMessage m *)
+  (*                                                   end) by (simpl; clean_map_lookups; trivial). *)
+  (*       rewrite <- RW; clear RW. *)
+  (*       erewrite key_perms_from_known_ciphers_user_new_cipher; eauto. *)
+  (*       rewrite merge_perms_sym with (ks1 := key_perms_from_known_ciphers cs mycs $0), <- merge_perms_assoc. *)
 
-        go; go.
-        eapply perm_merge_same with (ks1' := ks $k++ match c with
-                                                     | @SigCipher t0 _ _ _ m | @SigEncCipher t0 _ _ _ _ m => findKeysMessage m
-                                                     end); try eassumption; trivial; destruct c; rewrite merge_keys_mine; trivial.
-        rewrite RW; assumption.
+  (*       go; go. *)
+  (*       eapply perm_merge_same with (ks1' := ks $k++ match c with *)
+  (*                                                    | @SigCipher t0 _ _ _ m | @SigEncCipher t0 _ _ _ _ m => findKeysMessage m *)
+  (*                                                    end); try eassumption; trivial; destruct c; rewrite merge_keys_mine; trivial. *)
+  (*       rewrite RW; assumption. *)
 
-        repeat
-          match goal with
-          | [ H : _ $k++ _ $? _ = None |- _ ] => 
-            apply merge_perms_no_disappear_perms in H; split_ex
-          end.
-        repeat xx; eauto.
+  (*       repeat *)
+  (*         match goal with *)
+  (*         | [ H : _ $k++ _ $? _ = None |- _ ] =>  *)
+  (*           apply merge_perms_no_disappear_perms in H; split_ex *)
+  (*         end. *)
+  (*       repeat xx; eauto. *)
 
-    - invert H0; [ econstructor 1 | econstructor 2 ]; eauto; simpl in *; clean_map_lookups;
-        user_cipher_queues_prop;
-        msg_queue_prop;
-        (* erewrite <- key_perms_from_message_queue_idempotent_addnl_cipher; eauto; *)
-        erewrite <- key_perms_from_known_ciphers_idempotent_addnl_cipher; eauto.
-  Qed.
+  (*   - invert H0; [ econstructor 1 | econstructor 2 ]; eauto; simpl in *; clean_map_lookups; *)
+  (*       user_cipher_queues_prop; *)
+  (*       msg_queue_prop; *)
+  (*       (* erewrite <- key_perms_from_message_queue_idempotent_addnl_cipher; eauto; *) *)
+  (*       erewrite <- key_perms_from_known_ciphers_idempotent_addnl_cipher; eauto. *)
+  (* Qed. *)
 
-  Lemma message_eq_user_add_addnl_key :
-    forall A B (usrs : honest_users A) (adv adv' : user_data B) cs gks gks'
-      ks ks' kid k cmd qmsgs mycs froms sents cur_n cmd' sents' cur_n'
-      t (m__rw : crypto t) m__iw iu chid uid,
+  (* Lemma message_eq_user_add_addnl_key : *)
+  (*   forall A B (usrs : honest_users A) (adv adv' : user_data B) cs gks gks' *)
+  (*     ks ks' kid k cmd qmsgs mycs froms sents cur_n cmd' sents' cur_n' *)
+  (*     t (m__rw : crypto t) m__iw iu chid uid, *)
 
-      ~ In kid gks
-      -> ks' = add_key_perm kid true ks
-      -> gks' = gks $+ (kid,k)
-      -> usrs $? uid = Some (mkUserData ks cmd qmsgs mycs froms sents cur_n)
-      -> encrypted_ciphers_ok (findUserKeys usrs) cs gks
-      -> keys_and_permissions_good gks usrs adv.(key_heap)
-      (* -> user_cipher_queues_ok cs (findUserKeys usrs) usrs *)
-      -> message_queues_ok cs usrs gks
-      (* -> message_queue_ok (findUserKeys usrs) cs qmsgs gks *)
-      (* -> keys_mine ks (findKeysCrypto cs c) *)
-      -> message_eq m__rw {| users := usrs; adversary := adv; all_ciphers := cs; all_keys := gks |} m__iw iu chid
-      -> message_eq
-          m__rw
-          {| users :=
-               usrs $+ (uid,
-                        {| key_heap := ks';
-                           protocol := cmd';
-                           msg_heap := qmsgs;
-                           c_heap := mycs;
-                           from_nons := froms;
-                           sent_nons := sents';
-                           cur_nonce := cur_n' |});
-             adversary := adv';
-             all_ciphers := cs;
-             all_keys := gks' |} m__iw iu chid.
-  Proof.
-    intros; subst.
+  (*     ~ In kid gks *)
+  (*     -> ks' = add_key_perm kid true ks *)
+  (*     -> gks' = gks $+ (kid,k) *)
+  (*     -> usrs $? uid = Some (mkUserData ks cmd qmsgs mycs froms sents cur_n) *)
+  (*     -> encrypted_ciphers_ok (findUserKeys usrs) cs gks *)
+  (*     -> keys_and_permissions_good gks usrs adv.(key_heap) *)
+  (*     (* -> user_cipher_queues_ok cs (findUserKeys usrs) usrs *) *)
+  (*     -> message_queues_ok cs usrs gks *)
+  (*     (* -> message_queue_ok (findUserKeys usrs) cs qmsgs gks *) *)
+  (*     (* -> keys_mine ks (findKeysCrypto cs c) *) *)
+  (*     -> message_eq m__rw {| users := usrs; adversary := adv; all_ciphers := cs; all_keys := gks |} m__iw iu chid *)
+  (*     -> message_eq *)
+  (*         m__rw *)
+  (*         {| users := *)
+  (*              usrs $+ (uid, *)
+  (*                       {| key_heap := ks'; *)
+  (*                          protocol := cmd'; *)
+  (*                          msg_heap := qmsgs; *)
+  (*                          c_heap := mycs; *)
+  (*                          from_nons := froms; *)
+  (*                          sent_nons := sents'; *)
+  (*                          cur_nonce := cur_n' |}); *)
+  (*            adversary := adv'; *)
+  (*            all_ciphers := cs; *)
+  (*            all_keys := gks' |} m__iw iu chid. *)
+  (* Proof. *)
+  (*   intros; subst. *)
 
-    invert H6; [ econstructor 1 | econstructor 2 ]; simpl in *; eauto;
-      intros;
-      autorewrite with find_user_keys in *; eauto using message_content_eq_addnl_key;
-        destruct (u ==n uid); subst; clean_map_lookups; eauto; simpl; eauto;
-          assert (k__sign <> kid) by (encrypted_ciphers_prop; destruct (k__sign ==n kid); subst; clean_map_lookups; eauto);
-          clean_map_lookups;
-          match goal with
-          | [ ARG : ?usrs $? ?uid = Some _,
-                    IARG : IdealWorld.users _ $? ?uid = Some _,
-                           H : (forall _ _ _, ?usrs $? _ = Some _ -> _) |- _ ] =>
-            generalize ARG; intros; eapply H in ARG
-          end;
-          try
-            match goal with
-            | [ H : honest_key (?ks $+ (?kid1,_)) ?kid |- honest_key ?ks ?kid ] =>
-              assert (kid <> kid1) by (encrypted_ciphers_prop; destruct (kid ==n kid1); subst; clean_map_lookups; eauto);
-                invert H; constructor; clean_map_lookups; trivial
-            end; eauto.
+  (*   invert H6; [ econstructor 1 | econstructor 2 ]; simpl in *; eauto; *)
+  (*     intros; *)
+  (*     autorewrite with find_user_keys in *; eauto using message_content_eq_addnl_key; *)
+  (*       destruct (u ==n uid); subst; clean_map_lookups; eauto; simpl; eauto; *)
+  (*         assert (k__sign <> kid) by (encrypted_ciphers_prop; destruct (k__sign ==n kid); subst; clean_map_lookups; eauto); *)
+  (*         clean_map_lookups; *)
+  (*         match goal with *)
+  (*         | [ ARG : ?usrs $? ?uid = Some _, *)
+  (*                   IARG : IdealWorld.users _ $? ?uid = Some _, *)
+  (*                          H : (forall _ _ _, ?usrs $? _ = Some _ -> _) |- _ ] => *)
+  (*           generalize ARG; intros; eapply H in ARG *)
+  (*         end; *)
+  (*         try *)
+  (*           match goal with *)
+  (*           | [ H : honest_key (?ks $+ (?kid1,_)) ?kid |- honest_key ?ks ?kid ] => *)
+  (*             assert (kid <> kid1) by (encrypted_ciphers_prop; destruct (kid ==n kid1); subst; clean_map_lookups; eauto); *)
+  (*               invert H; constructor; clean_map_lookups; trivial *)
+  (*           end; eauto. *)
 
-    - invert H2; [ econstructor 1; swap 1 2 | econstructor 2; swap 1 2 ]; eauto; simpl in *; clean_map_lookups; eauto.
-      keys_and_permissions_prop.
-      unfold add_key_perm.
-      cases (ks $? kid).
-      apply H14 in Heq; clean_map_lookups.
-      msg_queue_prop.
-      (* erewrite <- key_perms_from_message_queue_idempotent_addnl_key; eauto. *)
-      eapply compat_perm_same; eauto.
+  (*   - invert H2; [ econstructor 1; swap 1 2 | econstructor 2; swap 1 2 ]; eauto; simpl in *; clean_map_lookups; eauto. *)
+  (*     keys_and_permissions_prop. *)
+  (*     unfold add_key_perm. *)
+  (*     cases (ks $? kid). *)
+  (*     apply H14 in Heq; clean_map_lookups. *)
+  (*     msg_queue_prop. *)
+  (*     (* erewrite <- key_perms_from_message_queue_idempotent_addnl_key; eauto. *) *)
+  (*     eapply compat_perm_same; eauto. *)
 
-    - invert H0; [ econstructor 1; swap 1 2 | econstructor 2; swap 1 2 ]; eauto; simpl in *; clean_map_lookups; eauto.
-      (* keys_and_permissions_prop. *)
-      (* unfold add_key_perm. *)
-      (* cases (data__rw.(key_heap) $? kid). *)
-      (* apply H16 in Heq; clean_map_lookups. *)
-      (* msg_queue_prop. *)
-      (* erewrite <- key_perms_from_message_queue_idempotent_addnl_key; eauto. *)
+  (*   - invert H0; [ econstructor 1; swap 1 2 | econstructor 2; swap 1 2 ]; eauto; simpl in *; clean_map_lookups; eauto. *)
+  (*     (* keys_and_permissions_prop. *) *)
+  (*     (* unfold add_key_perm. *) *)
+  (*     (* cases (data__rw.(key_heap) $? kid). *) *)
+  (*     (* apply H16 in Heq; clean_map_lookups. *) *)
+  (*     (* msg_queue_prop. *) *)
+  (*     (* erewrite <- key_perms_from_message_queue_idempotent_addnl_key; eauto. *) *)
 
-    - invert H2; [ econstructor 1; swap 1 2 | econstructor 2; swap 1 2 ];
-        eauto; simpl in *; clean_map_lookups; eauto;
-          keys_and_permissions_prop;
-          unfold add_key_perm;
-          cases (ks $? kid).
+  (*   - invert H2; [ econstructor 1; swap 1 2 | econstructor 2; swap 1 2 ]; *)
+  (*       eauto; simpl in *; clean_map_lookups; eauto; *)
+  (*         keys_and_permissions_prop; *)
+  (*         unfold add_key_perm; *)
+  (*         cases (ks $? kid). *)
 
-      apply H16 in Heq; clean_map_lookups.
+  (*     apply H16 in Heq; clean_map_lookups. *)
 
-      msg_queue_prop.
-      (* erewrite <- key_perms_from_message_queue_idempotent_addnl_key; eauto. *)
-      eapply compat_perm_same; eauto.
+  (*     msg_queue_prop. *)
+  (*     (* erewrite <- key_perms_from_message_queue_idempotent_addnl_key; eauto. *) *)
+  (*     eapply compat_perm_same; eauto. *)
 
-      apply H16 in Heq; clean_map_lookups.
+  (*     apply H16 in Heq; clean_map_lookups. *)
 
-      msg_queue_prop.
-      (* erewrite <- key_perms_from_message_queue_idempotent_addnl_key; eauto. *)
-      eapply compat_perm_same; eauto.
-      assert (k__enc0 <> kid) by (encrypted_ciphers_prop; destruct (k__enc0 ==n kid); subst; clean_map_lookups; eauto);
-        cases (kid ==n k__enc0); subst; clean_map_lookups; eauto.
+  (*     msg_queue_prop. *)
+  (*     (* erewrite <- key_perms_from_message_queue_idempotent_addnl_key; eauto. *) *)
+  (*     eapply compat_perm_same; eauto. *)
+  (*     assert (k__enc0 <> kid) by (encrypted_ciphers_prop; destruct (k__enc0 ==n kid); subst; clean_map_lookups; eauto); *)
+  (*       cases (kid ==n k__enc0); subst; clean_map_lookups; eauto. *)
 
-    - invert H0; [ econstructor 1; swap 1 2 | econstructor 2; swap 1 2 ]; eauto; simpl in *; clean_map_lookups; eauto;
-        keys_and_permissions_prop;
-        msg_queue_prop.
+  (*   - invert H0; [ econstructor 1; swap 1 2 | econstructor 2; swap 1 2 ]; eauto; simpl in *; clean_map_lookups; eauto; *)
+  (*       keys_and_permissions_prop; *)
+  (*       msg_queue_prop. *)
 
-      (* erewrite <- key_perms_from_message_queue_idempotent_addnl_key; eauto. *)
-      (* erewrite <- key_perms_from_message_queue_idempotent_addnl_key; eauto. *)
+  (*     (* erewrite <- key_perms_from_message_queue_idempotent_addnl_key; eauto. *) *)
+  (*     (* erewrite <- key_perms_from_message_queue_idempotent_addnl_key; eauto. *) *)
 
-  Qed.
+  (* Qed. *)
 
-  Lemma message_eq_user_decrypt_msg :
-    forall A B (usrs : honest_users A) (adv adv' : user_data B) cs gks
-      ks ks' cmd qmsgs mycs froms sents cur_n cmd' sents' cur_n'
-      t (m__rw : crypto t) m__iw iu chid uid cid k__s k__e uid' mseq t__m (msg : message t__m),
+  (* Lemma message_eq_user_decrypt_msg : *)
+  (*   forall A B (usrs : honest_users A) (adv adv' : user_data B) cs gks *)
+  (*     ks ks' cmd qmsgs mycs froms sents cur_n cmd' sents' cur_n' *)
+  (*     t (m__rw : crypto t) m__iw iu chid uid cid k__s k__e uid' mseq t__m (msg : message t__m), *)
 
-      cs $? cid = Some (SigEncCipher k__s k__e uid' mseq msg)
-      -> List.In cid mycs
-      -> ks' = ks $k++ findKeysMessage msg
-      -> usrs $? uid = Some (mkUserData ks cmd qmsgs mycs froms sents cur_n)
-      -> encrypted_ciphers_ok (findUserKeys usrs) cs gks
-      -> user_cipher_queues_ok cs (findUserKeys usrs) usrs
-      -> message_eq m__rw {| users := usrs; adversary := adv; all_ciphers := cs; all_keys := gks |} m__iw iu chid
-      -> message_eq
-          m__rw
-          {| users :=
-               usrs $+ (uid,
-                        {| key_heap := ks';
-                           protocol := cmd';
-                           msg_heap := qmsgs;
-                           c_heap := mycs;
-                           from_nons := froms;
-                           sent_nons := sents';
-                           cur_nonce := cur_n' |});
-             adversary := adv';
-             all_ciphers := cs;
-             all_keys := gks |} m__iw iu chid.
-  Proof.
-    intros; subst.
+  (*     cs $? cid = Some (SigEncCipher k__s k__e uid' mseq msg) *)
+  (*     -> List.In cid mycs *)
+  (*     -> ks' = ks $k++ findKeysMessage msg *)
+  (*     -> usrs $? uid = Some (mkUserData ks cmd qmsgs mycs froms sents cur_n) *)
+  (*     -> encrypted_ciphers_ok (findUserKeys usrs) cs gks *)
+  (*     -> user_cipher_queues_ok cs (findUserKeys usrs) usrs *)
+  (*     -> message_eq m__rw {| users := usrs; adversary := adv; all_ciphers := cs; all_keys := gks |} m__iw iu chid *)
+  (*     -> message_eq *)
+  (*         m__rw *)
+  (*         {| users := *)
+  (*              usrs $+ (uid, *)
+  (*                       {| key_heap := ks'; *)
+  (*                          protocol := cmd'; *)
+  (*                          msg_heap := qmsgs; *)
+  (*                          c_heap := mycs; *)
+  (*                          from_nons := froms; *)
+  (*                          sent_nons := sents'; *)
+  (*                          cur_nonce := cur_n' |}); *)
+  (*            adversary := adv'; *)
+  (*            all_ciphers := cs; *)
+  (*            all_keys := gks |} m__iw iu chid. *)
+  (* Proof. *)
+  (*   intros; subst. *)
 
-    assert (honest_key (findUserKeys usrs) k__s) by ( user_cipher_queues_prop; constructor; eauto ).
-    invert H1; encrypted_ciphers_prop; simpl in *; eauto.
+  (*   assert (honest_key (findUserKeys usrs) k__s) by ( user_cipher_queues_prop; constructor; eauto ). *)
+  (*   invert H1; encrypted_ciphers_prop; simpl in *; eauto. *)
 
-    invert H5; [ econstructor 1 | econstructor 2 ]; simpl in *; eauto;
-      intros;
-      autorewrite with find_user_keys in *; eauto;
-        destruct (u ==n uid); subst; clean_map_lookups; eauto; simpl; eauto;
-          match goal with
-          | [ ARG : ?usrs $? ?uid = Some _,
-                    IARG : IdealWorld.users _ $? ?uid = Some _,
-                           H : (forall _ _ _, ?usrs $? _ = Some _ -> _) |- _ ] =>
-            generalize ARG; intros; eapply H in ARG
-          end;
-          rewrite honestk_merge_new_msgs_keys_dec_same with (honestk := findUserKeys usrs) in * by eauto;
-          eauto.
+  (*   invert H5; [ econstructor 1 | econstructor 2 ]; simpl in *; eauto; *)
+  (*     intros; *)
+  (*     autorewrite with find_user_keys in *; eauto; *)
+  (*       destruct (u ==n uid); subst; clean_map_lookups; eauto; simpl; eauto; *)
+  (*         match goal with *)
+  (*         | [ ARG : ?usrs $? ?uid = Some _, *)
+  (*                   IARG : IdealWorld.users _ $? ?uid = Some _, *)
+  (*                          H : (forall _ _ _, ?usrs $? _ = Some _ -> _) |- _ ] => *)
+  (*           generalize ARG; intros; eapply H in ARG *)
+  (*         end; *)
+  (*         rewrite honestk_merge_new_msgs_keys_dec_same with (honestk := findUserKeys usrs) in * by eauto; *)
+  (*         eauto. *)
 
-    eapply ch_keys_from_cipher with (c_id' := cid); eauto; simpl; eauto.
-    eapply ch_keys_from_cipher with (c_id' := cid); eauto; simpl; eauto.
+  (*   eapply ch_keys_from_cipher with (c_id' := cid); eauto; simpl; eauto. *)
+  (*   eapply ch_keys_from_cipher with (c_id' := cid); eauto; simpl; eauto. *)
 
-  Qed.
+  (* Qed. *)
 
 
   (* Lemma message_eq_user_add : *)
@@ -1552,47 +1552,47 @@ Section MessageEqLemmas.
     unfold not; intros; clean_map_lookups.
   Qed.
 
-  Lemma message_eq_user_add_nochange_cs_ks_msgs_inv :
-    forall A B (usrs : honest_users A) (adv adv' : user_data B) cs gks
-      ks cmd qmsgs mycs froms sents cur_n cmd' sents' cur_n'
-      t (m__rw : crypto t) m__iw iu chid uid,
+  (* Lemma message_eq_user_add_nochange_cs_ks_msgs_inv : *)
+  (*   forall A B (usrs : honest_users A) (adv adv' : user_data B) cs gks *)
+  (*     ks cmd qmsgs mycs froms sents cur_n cmd' sents' cur_n' *)
+  (*     t (m__rw : crypto t) m__iw iu chid uid, *)
 
-      usrs $? uid = Some (mkUserData ks cmd qmsgs mycs froms sents cur_n)
-      -> message_eq
-          m__rw
-          {| users :=
-               usrs $+ (uid,
-                        {| key_heap := ks;
-                           protocol := cmd';
-                           msg_heap := qmsgs;
-                           c_heap := mycs;
-                           from_nons := froms;
-                           sent_nons := sents';
-                           cur_nonce := cur_n' |});
-             adversary := adv';
-             all_ciphers := cs;
-             all_keys := gks |} m__iw iu chid
-      -> message_eq m__rw {| users := usrs; adversary := adv; all_ciphers := cs; all_keys := gks |} m__iw iu chid.
-  Proof using All.
-    intros.
+  (*     usrs $? uid = Some (mkUserData ks cmd qmsgs mycs froms sents cur_n) *)
+  (*     -> message_eq *)
+  (*         m__rw *)
+  (*         {| users := *)
+  (*              usrs $+ (uid, *)
+  (*                       {| key_heap := ks; *)
+  (*                          protocol := cmd'; *)
+  (*                          msg_heap := qmsgs; *)
+  (*                          c_heap := mycs; *)
+  (*                          from_nons := froms; *)
+  (*                          sent_nons := sents'; *)
+  (*                          cur_nonce := cur_n' |}); *)
+  (*            adversary := adv'; *)
+  (*            all_ciphers := cs; *)
+  (*            all_keys := gks |} m__iw iu chid *)
+  (*     -> message_eq m__rw {| users := usrs; adversary := adv; all_ciphers := cs; all_keys := gks |} m__iw iu chid. *)
+  (* Proof using All. *)
+  (*   intros. *)
 
-    invert H0; [ econstructor 1 | econstructor 2 ]; simpl in *; eauto;
-      intros;
-      autorewrite with find_user_keys in *; eauto;
-        repeat
-          match goal with
-          | [ H : (forall _ _ _, _ $+ (?u,_) $? _ = Some _ -> _), IW : IdealWorld.users _ $? ?u = Some _ |- _ ] =>
-            specialize (H u); rewrite add_eq_o in H by trivial; specialize (H _ _ eq_refl IW)
-          | [ H : (forall _ _ _, _ $+ (?u1,_) $? _ = Some _ -> _), IW : IdealWorld.users _ $? ?u2 = Some _, NE : ?u1 <> ?u2 |- _ ] =>
-            specialize (H u2); rewrite add_neq_o in H by congruence; eapply H in IW; eauto
-          | [ H : (forall _ _ _, _ $+ (?uid1,_) $? _ = Some _ -> _), IW : IdealWorld.users _ $? ?u = Some _ |- _ ] =>
-            destruct (uid1 ==n u); subst; clean_map_lookups
-          end;
-        specialize_simply.
+  (*   invert H0; [ econstructor 1 | econstructor 2 ]; simpl in *; eauto; *)
+  (*     intros; *)
+  (*     autorewrite with find_user_keys in *; eauto; *)
+  (*       repeat *)
+  (*         match goal with *)
+  (*         | [ H : (forall _ _ _, _ $+ (?u,_) $? _ = Some _ -> _), IW : IdealWorld.users _ $? ?u = Some _ |- _ ] => *)
+  (*           specialize (H u); rewrite add_eq_o in H by trivial; specialize (H _ _ eq_refl IW) *)
+  (*         | [ H : (forall _ _ _, _ $+ (?u1,_) $? _ = Some _ -> _), IW : IdealWorld.users _ $? ?u2 = Some _, NE : ?u1 <> ?u2 |- _ ] => *)
+  (*           specialize (H u2); rewrite add_neq_o in H by congruence; eapply H in IW; eauto *)
+  (*         | [ H : (forall _ _ _, _ $+ (?uid1,_) $? _ = Some _ -> _), IW : IdealWorld.users _ $? ?u = Some _ |- _ ] => *)
+  (*           destruct (uid1 ==n u); subst; clean_map_lookups *)
+  (*         end; *)
+  (*       specialize_simply. *)
 
-    all: 
-      invert H11; [ econstructor 1 | econstructor 2 ]; eauto.
-  Qed.
+  (*   all:  *)
+  (*     invert H11; [ econstructor 1 | econstructor 2 ]; eauto. *)
+  (* Qed. *)
 
   (* Lemma message_eq_user_add_addnl_cipher_inv : *)
   (*   forall A B (usrs : honest_users A) (adv adv' : user_data B) cs cs' cid c gks *)
@@ -1676,170 +1676,170 @@ Section MessageEqLemmas.
   (*     eauto. *)
   (* Qed. *)
 
-  Lemma message_eq_user_add_addnl_key_inv :
-    forall A B (usrs : honest_users A) (adv adv' : user_data B) cs gks gks'
-      ks ks' kid k cmd qmsgs mycs froms sents cur_n cmd' sents' cur_n'
-      t (m__rw : crypto t) m__iw iu chid uid,
+  (* Lemma message_eq_user_add_addnl_key_inv : *)
+  (*   forall A B (usrs : honest_users A) (adv adv' : user_data B) cs gks gks' *)
+  (*     ks ks' kid k cmd qmsgs mycs froms sents cur_n cmd' sents' cur_n' *)
+  (*     t (m__rw : crypto t) m__iw iu chid uid, *)
 
-      ~ In kid gks
-      -> ks' = add_key_perm kid true ks
-      -> gks' = gks $+ (kid,k)
-      -> usrs $? uid = Some (mkUserData ks cmd qmsgs mycs froms sents cur_n)
-      -> encrypted_ciphers_ok (findUserKeys usrs) cs gks
-      -> keys_and_permissions_good gks usrs adv.(key_heap)
-      -> msg_honestly_signed (findUserKeys usrs) cs m__rw = true
-      -> message_queues_ok cs usrs gks
-      -> message_eq
-          m__rw
-          {| users :=
-               usrs $+ (uid,
-                        {| key_heap := ks';
-                           protocol := cmd';
-                           msg_heap := qmsgs;
-                           c_heap := mycs;
-                           from_nons := froms;
-                           sent_nons := sents';
-                           cur_nonce := cur_n' |});
-             adversary := adv';
-             all_ciphers := cs;
-             all_keys := gks' |} m__iw iu chid
-      -> message_eq m__rw {| users := usrs; adversary := adv; all_ciphers := cs; all_keys := gks |} m__iw iu chid.
-  Proof.
-    intros; subst.
+  (*     ~ In kid gks *)
+  (*     -> ks' = add_key_perm kid true ks *)
+  (*     -> gks' = gks $+ (kid,k) *)
+  (*     -> usrs $? uid = Some (mkUserData ks cmd qmsgs mycs froms sents cur_n) *)
+  (*     -> encrypted_ciphers_ok (findUserKeys usrs) cs gks *)
+  (*     -> keys_and_permissions_good gks usrs adv.(key_heap) *)
+  (*     -> msg_honestly_signed (findUserKeys usrs) cs m__rw = true *)
+  (*     -> message_queues_ok cs usrs gks *)
+  (*     -> message_eq *)
+  (*         m__rw *)
+  (*         {| users := *)
+  (*              usrs $+ (uid, *)
+  (*                       {| key_heap := ks'; *)
+  (*                          protocol := cmd'; *)
+  (*                          msg_heap := qmsgs; *)
+  (*                          c_heap := mycs; *)
+  (*                          from_nons := froms; *)
+  (*                          sent_nons := sents'; *)
+  (*                          cur_nonce := cur_n' |}); *)
+  (*            adversary := adv'; *)
+  (*            all_ciphers := cs; *)
+  (*            all_keys := gks' |} m__iw iu chid *)
+  (*     -> message_eq m__rw {| users := usrs; adversary := adv; all_ciphers := cs; all_keys := gks |} m__iw iu chid. *)
+  (* Proof. *)
+  (*   intros; subst. *)
 
-    invert H7; [ econstructor 1 | econstructor 2 ];
-      simpl in *;
-      autorewrite with find_user_keys in *;
-      eauto using message_content_eq_addnl_key_inv; intros.
+  (*   invert H7; [ econstructor 1 | econstructor 2 ]; *)
+  (*     simpl in *; *)
+  (*     autorewrite with find_user_keys in *; *)
+  (*     eauto using message_content_eq_addnl_key_inv; intros. *)
 
-    - pose proof (msg_honestly_signed_has_signing_key_cipher_id _ _ _ H5); split_ex.
-      pose proof (msg_honestly_signed_signing_key_honest _ _ _ H5 H0); simpl in *; clean_context.
-      cases (cs $? x); try discriminate; clean_context; simpl in *.
-      invert H7.
-      encrypted_ciphers_prop.
-      keys_and_permissions_prop.
-      eapply message_content_eq_addnl_key_inv; intros; eauto.
-      eapply H15 in H12; split_ex; subst.
-      eapply H9 in H12; split_ex; clean_map_lookups.
+  (*   - pose proof (msg_honestly_signed_has_signing_key_cipher_id _ _ _ H5); split_ex. *)
+  (*     pose proof (msg_honestly_signed_signing_key_honest _ _ _ H5 H0); simpl in *; clean_context. *)
+  (*     cases (cs $? x); try discriminate; clean_context; simpl in *. *)
+  (*     invert H7. *)
+  (*     encrypted_ciphers_prop. *)
+  (*     keys_and_permissions_prop. *)
+  (*     eapply message_content_eq_addnl_key_inv; intros; eauto. *)
+  (*     eapply H15 in H12; split_ex; subst. *)
+  (*     eapply H9 in H12; split_ex; clean_map_lookups. *)
 
-    - specialize (H16 u).
-      invert H7.
-      encrypted_ciphers_prop.
-      assert (PHG : permission_heap_good gks ks) by 
-          (clear H0; keys_and_permissions_prop; eauto).
-      cases ( ks $? kid ); try (apply PHG in Heq; split_ex; clean_map_lookups).
+  (*   - specialize (H16 u). *)
+  (*     invert H7. *)
+  (*     encrypted_ciphers_prop. *)
+  (*     assert (PHG : permission_heap_good gks ks) by  *)
+  (*         (clear H0; keys_and_permissions_prop; eauto). *)
+  (*     cases ( ks $? kid ); try (apply PHG in Heq; split_ex; clean_map_lookups). *)
 
-      destruct (uid ==n u); subst; clean_map_lookups; eauto.
+  (*     destruct (uid ==n u); subst; clean_map_lookups; eauto. *)
 
-      + eapply H16 in H1; eauto; context_map_rewrites.
-        invert H1; [ econstructor 1 | econstructor 2 ]; eauto; simpl in *; clean_map_lookups.
-        msg_queue_prop.
-        (* erewrite <- key_perms_from_message_queue_idempotent_addnl_key in H15 by eauto. *)
-        eapply compat_perm_same with (ks1 := ks $+ (kid,true)); eauto.
+  (*     + eapply H16 in H1; eauto; context_map_rewrites. *)
+  (*       invert H1; [ econstructor 1 | econstructor 2 ]; eauto; simpl in *; clean_map_lookups. *)
+  (*       msg_queue_prop. *)
+  (*       (* erewrite <- key_perms_from_message_queue_idempotent_addnl_key in H15 by eauto. *) *)
+  (*       eapply compat_perm_same with (ks1 := ks $+ (kid,true)); eauto. *)
 
-      + eapply H16 in H1; eauto; context_map_rewrites.
-        msg_queue_prop.
-        invert H1; [ econstructor 1 | econstructor 2 ]; eauto; simpl in *; clean_map_lookups; eauto.
-        (* erewrite <- key_perms_from_message_queue_idempotent_addnl_key in H20; eauto. *)
+  (*     + eapply H16 in H1; eauto; context_map_rewrites. *)
+  (*       msg_queue_prop. *)
+  (*       invert H1; [ econstructor 1 | econstructor 2 ]; eauto; simpl in *; clean_map_lookups; eauto. *)
+  (*       (* erewrite <- key_perms_from_message_queue_idempotent_addnl_key in H20; eauto. *) *)
 
-    - pose proof (msg_honestly_signed_has_signing_key_cipher_id _ _ _ H5); split_ex.
-      pose proof (msg_honestly_signed_signing_key_honest _ _ _ H5 H0); simpl in *; clean_context.
-      cases (cs $? x); try discriminate; clean_context; simpl in *.
-      invert H7.
-      encrypted_ciphers_prop.
-      keys_and_permissions_prop.
-      eapply message_content_eq_addnl_key_inv; intros; eauto.
-      eapply H19 in H11; split_ex; subst.
-      eapply H9 in H11; split_ex; clean_map_lookups.
+  (*   - pose proof (msg_honestly_signed_has_signing_key_cipher_id _ _ _ H5); split_ex. *)
+  (*     pose proof (msg_honestly_signed_signing_key_honest _ _ _ H5 H0); simpl in *; clean_context. *)
+  (*     cases (cs $? x); try discriminate; clean_context; simpl in *. *)
+  (*     invert H7. *)
+  (*     encrypted_ciphers_prop. *)
+  (*     keys_and_permissions_prop. *)
+  (*     eapply message_content_eq_addnl_key_inv; intros; eauto. *)
+  (*     eapply H19 in H11; split_ex; subst. *)
+  (*     eapply H9 in H11; split_ex; clean_map_lookups. *)
 
-    - specialize (H16 u).
-      invert H7.
-      invert H8.
-      encrypted_ciphers_prop.
-      assert (PHG : permission_heap_good gks ks) by 
-          (clear H0; keys_and_permissions_prop; eauto).
-      cases ( ks $? kid ); try (apply PHG in Heq; split_ex; clean_map_lookups).
+  (*   - specialize (H16 u). *)
+  (*     invert H7. *)
+  (*     invert H8. *)
+  (*     encrypted_ciphers_prop. *)
+  (*     assert (PHG : permission_heap_good gks ks) by  *)
+  (*         (clear H0; keys_and_permissions_prop; eauto). *)
+  (*     cases ( ks $? kid ); try (apply PHG in Heq; split_ex; clean_map_lookups). *)
 
-      destruct (uid ==n u); subst; clean_map_lookups; eauto.
+  (*     destruct (uid ==n u); subst; clean_map_lookups; eauto. *)
 
-      + eapply H16 in H1; eauto; context_map_rewrites.
-        msg_queue_prop.
-        invert H1; simpl in *; [ econstructor 1 | econstructor 2; swap 1 2 ]; eauto; simpl;
-          (* erewrite <- key_perms_from_message_queue_idempotent_addnl_key in * by eauto; *)
-          clean_map_lookups.
+  (*     + eapply H16 in H1; eauto; context_map_rewrites. *)
+  (*       msg_queue_prop. *)
+  (*       invert H1; simpl in *; [ econstructor 1 | econstructor 2; swap 1 2 ]; eauto; simpl; *)
+  (*         (* erewrite <- key_perms_from_message_queue_idempotent_addnl_key in * by eauto; *) *)
+  (*         clean_map_lookups. *)
 
-        eapply compat_perm_same with (ks1 := ks $+ (kid,true)); eauto.
-        eapply compat_perm_same with (ks1 := ks $+ (kid,true)); eauto.
+  (*       eapply compat_perm_same with (ks1 := ks $+ (kid,true)); eauto. *)
+  (*       eapply compat_perm_same with (ks1 := ks $+ (kid,true)); eauto. *)
 
-      + eapply H16 in H1; eauto; context_map_rewrites.
-        msg_queue_prop.
-        invert H1; [ econstructor 1 | econstructor 2; swap 1 2 ]; eauto; clean_map_lookups; simpl in *;
-          erewrite <- key_perms_from_message_queue_idempotent_addnl_key in * by eauto; eauto.
+  (*     + eapply H16 in H1; eauto; context_map_rewrites. *)
+  (*       msg_queue_prop. *)
+  (*       invert H1; [ econstructor 1 | econstructor 2; swap 1 2 ]; eauto; clean_map_lookups; simpl in *; *)
+  (*         erewrite <- key_perms_from_message_queue_idempotent_addnl_key in * by eauto; eauto. *)
 
-        Unshelve.
-        all: auto.
-  Qed.
+  (*       Unshelve. *)
+  (*       all: auto. *)
+  (* Qed. *)
 
-  Lemma message_eq_user_decrypt_msg_inv :
-    forall A B (usrs : honest_users A) (adv adv' : user_data B) cs gks
-      ks ks' cmd qmsgs mycs froms sents cur_n cmd' sents' cur_n'
-      t (m__rw : crypto t) m__iw iu chid uid cid k__s k__e uid' mseq t__m (msg : message t__m),
+  (* Lemma message_eq_user_decrypt_msg_inv : *)
+  (*   forall A B (usrs : honest_users A) (adv adv' : user_data B) cs gks *)
+  (*     ks ks' cmd qmsgs mycs froms sents cur_n cmd' sents' cur_n' *)
+  (*     t (m__rw : crypto t) m__iw iu chid uid cid k__s k__e uid' mseq t__m (msg : message t__m), *)
 
-      cs $? cid = Some (SigEncCipher k__s k__e uid' mseq msg)
-      -> List.In cid mycs
-      -> ks' = ks $k++ findKeysMessage msg
-      -> usrs $? uid = Some (mkUserData ks cmd qmsgs mycs froms sents cur_n)
-      -> encrypted_ciphers_ok (findUserKeys usrs) cs gks
-      -> user_cipher_queues_ok cs (findUserKeys usrs) usrs
-      -> message_eq
-          m__rw
-          {| users :=
-               usrs $+ (uid,
-                        {| key_heap := ks';
-                           protocol := cmd';
-                           msg_heap := qmsgs;
-                           c_heap := mycs;
-                           from_nons := froms;
-                           sent_nons := sents';
-                           cur_nonce := cur_n' |});
-             adversary := adv';
-             all_ciphers := cs;
-             all_keys := gks |} m__iw iu chid
-      -> message_eq m__rw {| users := usrs; adversary := adv; all_ciphers := cs; all_keys := gks |} m__iw iu chid.
-  Proof.
-    intros.
+  (*     cs $? cid = Some (SigEncCipher k__s k__e uid' mseq msg) *)
+  (*     -> List.In cid mycs *)
+  (*     -> ks' = ks $k++ findKeysMessage msg *)
+  (*     -> usrs $? uid = Some (mkUserData ks cmd qmsgs mycs froms sents cur_n) *)
+  (*     -> encrypted_ciphers_ok (findUserKeys usrs) cs gks *)
+  (*     -> user_cipher_queues_ok cs (findUserKeys usrs) usrs *)
+  (*     -> message_eq *)
+  (*         m__rw *)
+  (*         {| users := *)
+  (*              usrs $+ (uid, *)
+  (*                       {| key_heap := ks'; *)
+  (*                          protocol := cmd'; *)
+  (*                          msg_heap := qmsgs; *)
+  (*                          c_heap := mycs; *)
+  (*                          from_nons := froms; *)
+  (*                          sent_nons := sents'; *)
+  (*                          cur_nonce := cur_n' |}); *)
+  (*            adversary := adv'; *)
+  (*            all_ciphers := cs; *)
+  (*            all_keys := gks |} m__iw iu chid *)
+  (*     -> message_eq m__rw {| users := usrs; adversary := adv; all_ciphers := cs; all_keys := gks |} m__iw iu chid. *)
+  (* Proof. *)
+  (*   intros. *)
 
-    invert H5; [ econstructor 1 | econstructor 2 ]; simpl in *; eauto;
-      autorewrite with find_user_keys in *;
-      (* destruct (cid ==n c_id); subst; clean_map_lookups; trivial; *)
-      intros;
-      repeat
-        match goal with
-        | [ H : (forall _ _ _, _ $+ (?u,_) $? _ = Some _ -> _), IW : IdealWorld.users _ $? ?u = Some _ |- _ ] =>
-          specialize (H u); rewrite add_eq_o in H by trivial; specialize (H _ _ eq_refl IW)
-        | [ H : (forall _ _ _, _ $+ (?u1,_) $? _ = Some _ -> _), IW : IdealWorld.users _ $? ?u2 = Some _, NE : ?u1 <> ?u2 |- _ ] =>
-          specialize (H u2); rewrite add_neq_o in H by congruence; eapply H in IW; eauto
-        | [ H : (forall _ _ _, _ $+ (?uid1,_) $? _ = Some _ -> _), IW : IdealWorld.users _ $? ?u = Some _ |- _ ] =>
-          destruct (uid1 ==n u); subst; clean_map_lookups
-        | [ HK : honest_key ?honk ?k, H : honest_key (?honk $k++ ?newk) ?k -> _ |- _ ] =>
-          assert (honest_key (honk $k++ newk) k) by eauto using honest_key_after_new_keys; specialize_simply
-        end; eauto using honest_key_after_new_keys.
+  (*   invert H5; [ econstructor 1 | econstructor 2 ]; simpl in *; eauto; *)
+  (*     autorewrite with find_user_keys in *; *)
+  (*     (* destruct (cid ==n c_id); subst; clean_map_lookups; trivial; *) *)
+  (*     intros; *)
+  (*     repeat *)
+  (*       match goal with *)
+  (*       | [ H : (forall _ _ _, _ $+ (?u,_) $? _ = Some _ -> _), IW : IdealWorld.users _ $? ?u = Some _ |- _ ] => *)
+  (*         specialize (H u); rewrite add_eq_o in H by trivial; specialize (H _ _ eq_refl IW) *)
+  (*       | [ H : (forall _ _ _, _ $+ (?u1,_) $? _ = Some _ -> _), IW : IdealWorld.users _ $? ?u2 = Some _, NE : ?u1 <> ?u2 |- _ ] => *)
+  (*         specialize (H u2); rewrite add_neq_o in H by congruence; eapply H in IW; eauto *)
+  (*       | [ H : (forall _ _ _, _ $+ (?uid1,_) $? _ = Some _ -> _), IW : IdealWorld.users _ $? ?u = Some _ |- _ ] => *)
+  (*         destruct (uid1 ==n u); subst; clean_map_lookups *)
+  (*       | [ HK : honest_key ?honk ?k, H : honest_key (?honk $k++ ?newk) ?k -> _ |- _ ] => *)
+  (*         assert (honest_key (honk $k++ newk) k) by eauto using honest_key_after_new_keys; specialize_simply *)
+  (*       end; eauto using honest_key_after_new_keys. *)
 
-    clear H13; user_cipher_queues_prop; encrypted_ciphers_prop;
-      rewrite honestk_merge_new_msgs_keys_dec_same with (honestk := findUserKeys usrs) in * by eauto.
-    eapply ch_keys_from_cipher_inv with (c_id' := cid); simpl; eauto.
+  (*   clear H13; user_cipher_queues_prop; encrypted_ciphers_prop; *)
+  (*     rewrite honestk_merge_new_msgs_keys_dec_same with (honestk := findUserKeys usrs) in * by eauto. *)
+  (*   eapply ch_keys_from_cipher_inv with (c_id' := cid); simpl; eauto. *)
 
 
-    clear H1 H13; user_cipher_queues_prop; encrypted_ciphers_prop;
-      rewrite honestk_merge_new_msgs_keys_dec_same with (honestk := findUserKeys usrs) in * by eauto; eauto.
+  (*   clear H1 H13; user_cipher_queues_prop; encrypted_ciphers_prop; *)
+  (*     rewrite honestk_merge_new_msgs_keys_dec_same with (honestk := findUserKeys usrs) in * by eauto; eauto. *)
 
-    clear H13; user_cipher_queues_prop; encrypted_ciphers_prop;
-      rewrite honestk_merge_new_msgs_keys_dec_same with (honestk := findUserKeys usrs) in * by eauto.
-    eapply ch_keys_from_cipher_inv with (c_id' := cid); simpl; eauto.
+  (*   clear H13; user_cipher_queues_prop; encrypted_ciphers_prop; *)
+  (*     rewrite honestk_merge_new_msgs_keys_dec_same with (honestk := findUserKeys usrs) in * by eauto. *)
+  (*   eapply ch_keys_from_cipher_inv with (c_id' := cid); simpl; eauto. *)
     
-    clear H1 H13; user_cipher_queues_prop; encrypted_ciphers_prop;
-      rewrite honestk_merge_new_msgs_keys_dec_same with (honestk := findUserKeys usrs) in * by eauto; eauto.
-  Qed.
+  (*   clear H1 H13; user_cipher_queues_prop; encrypted_ciphers_prop; *)
+  (*     rewrite honestk_merge_new_msgs_keys_dec_same with (honestk := findUserKeys usrs) in * by eauto; eauto. *)
+  (* Qed. *)
 
 
 End MessageEqLemmas.
